erasure/theories/ErasureCorrectness.v
@@ -143,8 +143,8 @@ Proof.
     eapply typing_wf_local in a1. subst types.
     2:eauto.
 
-    eapply All_local_env_app_inv.
-    eapply All_local_env_app in a1. intuition auto.
+    eapply All_local_env_app.
+    eapply All_local_env_app_inv in a1. intuition auto.
 
     (* clear -wfΣ X2 a2 b4 X1. *)
     eapply All_local_env_impl; eauto. simpl; intros.
@@ -154,7 +154,7 @@ Proof.
     eapply typing_wf_local in X3.
     eapply PCUICSafeChecker.wf_local_app_inv.
     eauto. eapply wf_local_rel_local in X3.
-    eapply wf_local_rel_app in X3 as []. rewrite app_context_nil_l in w0.
+    eapply wf_local_rel_app_inv in X3 as []. rewrite app_context_nil_l in w0.
     eapply wf_local_rel_conv; eauto.
     destruct X3. exists x0.
     eapply PCUICContextConversion.context_conversion with (Γ ,,, Γ0); eauto.
@@ -163,7 +163,7 @@ Proof.
     eapply typing_wf_local in t0.
     eapply PCUICSafeChecker.wf_local_app_inv.
     eauto. eapply wf_local_rel_local in t0.
-    eapply wf_local_rel_app in t0 as []. rewrite app_context_nil_l in w0.
+    eapply wf_local_rel_app_inv in t0 as []. rewrite app_context_nil_l in w0.
     eapply wf_local_rel_conv; eauto.
   - econstructor.
 
@@ -176,8 +176,8 @@ Proof.
     eapply typing_wf_local in a0. subst types.
     2:eauto.
 
-    eapply All_local_env_app_inv.
-    eapply All_local_env_app in a0. intuition auto.
+    eapply All_local_env_app.
+    eapply All_local_env_app_inv in a0. intuition auto.
 
     (* clear -wfΣ X2 a2 b4 X1. *)
     eapply All_local_env_impl; eauto. simpl; intros.
@@ -187,7 +187,7 @@ Proof.
     eapply typing_wf_local in X3.
     eapply PCUICSafeChecker.wf_local_app_inv.
     eauto. eapply wf_local_rel_local in X3.
-    eapply wf_local_rel_app in X3 as []. rewrite app_context_nil_l in w0.
+    eapply wf_local_rel_app_inv in X3 as []. rewrite app_context_nil_l in w0.
 
 
     eapply wf_local_rel_conv; eauto.
@@ -198,7 +198,7 @@ Proof.
     eapply typing_wf_local in t0.
     eapply PCUICSafeChecker.wf_local_app_inv.
     eauto. eapply wf_local_rel_local in t0.
-    eapply wf_local_rel_app in t0 as []. rewrite app_context_nil_l in w0.
+    eapply wf_local_rel_app_inv in t0 as []. rewrite app_context_nil_l in w0.
     eapply wf_local_rel_conv; eauto.
 Qed.
 
