pcuic/theories/PCUICSpine.v
@@ -325,12 +325,12 @@ Proof.
         specialize (IHn (subst_context [b] 0 l)).
         forward IHn. {
           rewrite app_context_assoc in wfΓ'.
-          apply All_local_env_app in wfΓ' as [wfb wfa].
+          apply All_local_env_app_inv in wfΓ' as [wfb wfa].
           depelim wfb.
           eapply substitution_wf_local. eauto. 
           epose proof (cons_let_def Σ Γ [] [] na b ty ltac:(constructor)).
           rewrite !subst_empty in X. eapply X. auto.
-          eapply All_local_env_app_inv; split.
+          eapply All_local_env_app; split.
           constructor; auto. apply wfa. }
         forward IHn by rewrite subst_context_length; lia.
         specialize (IHn s inst s' Hsp). 
@@ -359,14 +359,14 @@ Proof.
         specialize (IHn (subst_context [hd] 0 l)).
         forward IHn. {
           rewrite app_context_assoc in wfΓ'.
-          apply All_local_env_app in wfΓ' as [wfb wfa]; eauto.
+          apply All_local_env_app_inv in wfΓ' as [wfb wfa]; eauto.
           depelim wfb. 
           eapply substitution_wf_local. auto. 
           constructor. constructor. rewrite subst_empty.
           eapply type_Cumul'. eapply t.
           eapply l0.
           eapply conv_cumul; auto. now symmetry. 
-          eapply All_local_env_app_inv; eauto; split.
+          eapply All_local_env_app; eauto; split.
           constructor; eauto. eapply isType_tProd in i; intuition eauto. }
         forward IHn by rewrite subst_context_length; lia.
         specialize (IHn s tl s'). 
@@ -650,7 +650,7 @@ Proof.
   rewrite firstn_0 in csr => //. rewrite app_nil_r in csr.
   eapply subslet_app_inv in subs as [sl sr].
   split; split; auto. rewrite app_context_assoc in wfcodom.
-  now eapply All_local_env_app in wfcodom as [? ?].
+  now eapply All_local_env_app_inv in wfcodom as [? ?].
   eapply substitution_wf_local; eauto.
   now rewrite app_context_assoc in wfcodom.
 Qed.
@@ -1721,8 +1721,8 @@ Proof.
       * eapply subslet_app => //. eapply sps.
         rewrite -{1}(subst_empty 0 b).
         repeat constructor. rewrite !subst_empty.
-        eapply All_local_env_app in wfΓΔ as [_ wf].
-        eapply All_local_env_app in wf as [wfd _].
+        eapply All_local_env_app_inv in wfΓΔ as [_ wf].
+        eapply All_local_env_app_inv in wf as [wfd _].
         depelim wfd. apply l0.
       * rewrite subst_app_simpl.
         move: (context_subst_length sps).
@@ -1747,7 +1747,7 @@ Proof.
       2:{ eauto. }
       forward X. {
         pose proof wfΓΔ as wfΓΔ'.
-        rewrite app_context_assoc in wfΓΔ'. eapply All_local_env_app in wfΓΔ' as [wfΓΔ' _].
+        rewrite app_context_assoc in wfΓΔ'. eapply All_local_env_app_inv in wfΓΔ' as [wfΓΔ' _].
         eapply (isType_subst wfΣ wfΓΔ') in wat''; eauto.
         2:{ repeat constructor. now rewrite subst_empty. }
         now rewrite subst_it_mkProd_or_LetIn Nat.add_0_r in wat''. }
@@ -1889,7 +1889,7 @@ Proof.
     simpl. rewrite smash_context_acc. simpl. auto.
     auto. }
   split; auto.
-  - eapply All_local_env_app_inv; split; auto.
+  - eapply All_local_env_app; split; auto.
     eapply wf_local_rel_smash_context; auto.
   - induction inst_subslet0 in inst, inst_ctx_subst0, spine_codom_wf0 |- *.
     depelim inst_ctx_subst0.
